Relaxed finiteness requirement for search space; however the generalized worklist algorithm is now less general than before

Unified_PW.thy
@@ -45,11 +45,15 @@ begin
     shows "reachable a'"
   using assms unfolding reachable_def by simp
 
-
   lemma finitely_branching:
     assumes "reachable a"
-    shows "finite (Collect (E a))"
-    by (metis assms finite_reachable finite_subset mem_Collect_eq step_reachable subsetI)
+    shows "finite ({a'. E a a' \<and> \<not> empty a'})"
+  proof -
+    have "{a'. E a a' \<and> \<not> empty a'} \<subseteq> {a'. reachable a' \<and> \<not> empty a'}"
+      using assms(1) by (auto intro: step_reachable)
+    then show ?thesis using finite_reachable
+      by (rule finite_subset)
+  qed
 
 end -- \<open>Search Space\<close>
 
@@ -57,7 +61,7 @@ subsection \<open>Generalized Worklist Algorithm\<close>
 
 context Search_Space_Defs_Empty
 begin
-  definition "reachable_subsumed S = {x' | x x'. reachable x' \<and> x' \<preceq> x \<and> x \<in> S}"
+  definition "reachable_subsumed S = {x' | x x'. reachable x' \<and> \<not> empty x' \<and> x' \<preceq> x \<and> x \<in> S}"
 
   definition
     "pw_var =
@@ -65,7 +69,7 @@ begin
       {(b, b'). b \<and> \<not> b'}
         <*lex*>
       {(passed', passed).
-        passed' \<subseteq> Collect reachable \<and> passed \<subseteq> Collect reachable \<and>
+        passed' \<subseteq> {a. reachable a \<and> \<not> empty a} \<and> passed \<subseteq> {a. reachable a \<and> \<not> empty a} \<and>
         reachable_subsumed passed \<subset> reachable_subsumed passed'}
         <*lex*>
       measure size
@@ -77,12 +81,12 @@ begin
     (\<forall> a \<in> passed. (\<exists> a' \<in> set_mset wait. a \<preceq> a') \<or>
     (\<forall> a'. E a a' \<and> \<not> empty a' \<longrightarrow> (\<exists> b' \<in> passed \<union> set_mset wait. a' \<preceq> b')))"
 
-  definition "start_subsumed passed wait = (\<exists> a \<in> passed \<union> set_mset wait. a\<^sub>0 \<preceq> a)"
+  definition "start_subsumed passed wait = (\<not> empty a\<^sub>0 \<longrightarrow> (\<exists> a \<in> passed \<union> set_mset wait. a\<^sub>0 \<preceq> a))"
 
   definition "pw_inv \<equiv> \<lambda> (passed, wait, brk).
     (brk \<longrightarrow> (\<exists> f. reachable f \<and> F f)) \<and>
     (\<not> brk \<longrightarrow>
-      passed \<subseteq> Collect reachable
+      passed \<subseteq> {a. reachable a \<and> \<not> empty a}
     \<and> pw_inv_frontier passed wait
     \<and> (\<forall> a \<in> passed \<union> set_mset wait. \<not> F a)
     \<and> start_subsumed passed wait
@@ -97,12 +101,15 @@ begin
       (\<forall> s \<in> set_mset wait. \<exists> s' \<in> set_mset wait'. s \<preceq> s') \<and>
       (\<forall> s \<in> {a' . E a a' \<and> \<not> empty a'}. \<exists> s' \<in> set_mset wait' \<union> passed. s \<preceq> s') \<and>
       (\<forall> s \<in> passed \<union> {a}. \<exists> s' \<in> passed'. s \<preceq> s') \<and>
-      (passed' \<subseteq> passed \<union> {a} \<union> {a' . E a a'} \<and>
+      (passed' \<subseteq> passed \<union> {a} \<union> {a' . E a a' \<and> \<not> empty a'} \<and>
       ((\<exists> x \<in> passed'. \<not> (\<exists> x' \<in> passed. x \<preceq> x')) \<or> wait' \<subseteq># wait \<and> passed = passed')
       )
   )"
 
-  definition "init_pw_spec \<equiv> SPEC (\<lambda> (passed, wait). wait = {#a\<^sub>0#} \<and> passed \<subseteq> {a\<^sub>0})"
+  definition
+    "init_pw_spec \<equiv>
+      SPEC (\<lambda> (passed, wait).
+        if empty a\<^sub>0 then passed = {} \<and> wait \<subseteq># {#a\<^sub>0#} else passed \<subseteq> {a\<^sub>0} \<and> wait = {#a\<^sub>0#})"
 
   abbreviation subsumed_elem :: "'a \<Rightarrow> 'a set \<Rightarrow> bool"
     where "subsumed_elem a M \<equiv> \<exists> a'. a' \<in> M \<and> a \<preceq> a'"
@@ -134,6 +141,7 @@ begin
     "pw_algo = do
       {
         if F a\<^sub>0 then RETURN True
+        else if empty a\<^sub>0 then RETURN False
         else do {
           (passed, wait) \<leftarrow> init_pw_spec;
           (passed, wait, brk) \<leftarrow> WHILEIT pw_inv (\<lambda> (passed, wait, brk). \<not> brk \<and> wait \<noteq> {#})
@@ -141,7 +149,7 @@ begin
               {
                 (a, wait) \<leftarrow> take_from_mset wait;
                 ASSERT (reachable a);
-                add_pw_spec passed wait a
+                if empty a then RETURN (passed, wait, brk) else add_pw_spec passed wait a
               }
             )
             (passed, wait, False);
@@ -154,18 +162,19 @@ end
 
 subsubsection \<open>Correctness Proof\<close>
 
-context Search_Space begin
+context Search_Space' begin
 
   lemma wf_worklist_var_aux:
     "wf {(passed', passed).
-      passed' \<subseteq> Collect reachable \<and> passed \<subseteq> Collect reachable \<and>
+      passed' \<subseteq> {a. reachable a \<and> \<not> empty a} \<and> passed \<subseteq> {a. reachable a \<and> \<not> empty a} \<and>
       reachable_subsumed passed \<subset> reachable_subsumed passed'}"
   proof (rule finite_acyclic_wf, goal_cases)
     case 1
     have "{(passed', passed).
-        passed' \<subseteq> Collect reachable \<and> passed \<subseteq> Collect reachable \<and>
+        passed' \<subseteq> {a. reachable a \<and> \<not> empty a} \<and> passed \<subseteq> {a. reachable a \<and> \<not> empty a} \<and>
         reachable_subsumed passed \<subset> reachable_subsumed passed'}
-        \<subseteq> {(passed', passed). passed \<subseteq> Collect reachable \<and> passed' \<subseteq> Collect reachable}"
+   \<subseteq> {(passed', passed).
+        passed \<subseteq> {a. reachable a \<and> \<not> empty a} \<and> passed' \<subseteq> {a. reachable a \<and> \<not> empty a}}"
       unfolding reachable_subsumed_def by auto
     moreover have "finite \<dots>" using finite_reachable using [[simproc add: finite_Collect]] by simp
     ultimately show ?case by (rule finite_subset)
@@ -174,7 +183,8 @@ context Search_Space begin
     show ?case
     proof (rule acyclicI_order[where f = "\<lambda> a. card (reachable_subsumed a)"], rule psubset_card_mono)
       fix a
-      have "reachable_subsumed a \<subseteq> Collect reachable" unfolding reachable_subsumed_def by blast
+      have "reachable_subsumed a \<subseteq> {a. reachable a \<and> \<not> empty a}"
+        unfolding reachable_subsumed_def by blast
       then show "finite (reachable_subsumed a)" using finite_reachable by (rule finite_subset)
     qed auto
   qed
@@ -198,7 +208,15 @@ context Search_Space begin
       "\<forall>s\<in>#wait - {#a#}. Multiset.Bex wait' (op \<preceq> s)"
     shows "start_subsumed passed' wait'"
       using assms unfolding start_subsumed_def apply clarsimp
-    by (metis Un_iff insert_DiffM2 local.trans mset_right_cancel_elem)
+      by (metis Un_iff insert_DiffM2 local.trans mset_right_cancel_elem)
+
+  private lemma aux11:
+    assumes
+      "empty a"
+      "start_subsumed passed wait"
+    shows "start_subsumed passed (wait - {#a#})"
+      using assms unfolding start_subsumed_def
+      by auto (metis UnI2 diff_single_trivial empty_mono insert_DiffM insert_noteq_member)
 
   lemma aux3_aux:
     assumes "pw_inv_frontier' passed wait"
@@ -206,7 +224,7 @@ context Search_Space begin
       "E b b'"
       "\<not> empty b" "\<not> empty b'"
       "b \<in>' passed"
-      "reachable b" "passed \<subseteq> Collect reachable"
+      "reachable b" "passed \<subseteq> {a. reachable a \<and> \<not> empty a}"
     shows "b' \<in>' passed \<union> set_mset wait"
   proof -
     from \<open>b \<in>' _\<close> obtain b1 where b1: "b \<preceq> b1" "b1 \<in> passed"
@@ -225,6 +243,14 @@ context Search_Space begin
   qed
 
 
+  private lemma pw_inv_frontier_empty_elem:
+    assumes "pw_inv_frontier passed wait" "passed \<subseteq> {a. reachable a \<and> \<not> empty a}" "empty a"
+    shows "pw_inv_frontier passed (wait - {#a#})"
+    using assms
+    unfolding pw_inv_frontier_def
+      apply auto
+    by (smt UnCI UnE diff_single_trivial empty_mono insert_DiffM2 mset_cancel_elem(1) subset_Collect_conv)
+
   private lemma aux3:
     assumes
       "set_mset wait \<subseteq> Collect reachable"
@@ -232,9 +258,9 @@ context Search_Space begin
       "\<forall> s \<in> set_mset (wait - {#a#}). \<exists> s' \<in> set_mset wait'. s \<preceq> s'"
       "\<forall> s \<in> {a'. E a a' \<and> \<not> empty a'}. \<exists> s' \<in> passed \<union> set_mset wait'. s \<preceq> s'"
       "\<forall> s \<in> passed \<union> {a}. \<exists> s' \<in> passed'. s \<preceq> s'"
-      "passed' \<subseteq> passed \<union> {a} \<union> {a' . E a a'}"
+      "passed' \<subseteq> passed \<union> {a} \<union> {a' . E a a' \<and> \<not> empty a}"
       "pw_inv_frontier passed wait"
-      "passed \<subseteq> Collect reachable"
+      "passed \<subseteq> {a. reachable a \<and> \<not> empty a}"
     shows "pw_inv_frontier passed' wait'"
   proof -
     from assms(1,2) have "reachable a"
@@ -247,7 +273,7 @@ context Search_Space begin
       "\<forall> s. s \<in>' passed \<union> {a} \<longrightarrow> s \<in>' passed'"
       "passed' \<subseteq> passed \<union> {a} \<union> {a' . E a a'}"
       "pw_inv_frontier' passed wait"
-      "passed \<subseteq> Collect reachable"
+      "passed \<subseteq> {a. reachable a \<and> \<not> empty a}"
       by (blast intro: trans pw_inv_frontier_frontier')+
 
     show ?thesis unfolding pw_inv_frontier_def
@@ -288,7 +314,9 @@ context Search_Space begin
           from 2 \<open>\<not> b \<in>' set_mset wait'\<close> assms'(2,3) have "\<not> b \<in>' set_mset wait"
             by (metis insert_DiffM2 mset_right_cancel_elem)
           from
-            aux3_aux[OF assms'(7) this \<open>E b b'\<close> \<open>\<not> empty b\<close> \<open>\<not> empty b'\<close> \<open>b \<in>' passed\<close> \<open>reachable b\<close> assms'(8)]
+            aux3_aux[OF
+              assms'(7) this \<open>E b b'\<close> \<open>\<not> empty b\<close> \<open>\<not> empty b'\<close> \<open>b \<in>' passed\<close> \<open>reachable b\<close> assms'(8)
+              ]
           have "b' \<in>' passed \<union> set_mset wait" .
           with assms'(2,3,5) show ?thesis
             by auto (metis insert_DiffM insert_noteq_member)
@@ -328,11 +356,12 @@ context Search_Space begin
 
   lemma aux4:
     assumes "pw_inv_frontier passed {#}" "reachable x" "start_subsumed passed {#}"
-            "passed \<subseteq> Collect reachable"
+            "passed \<subseteq> {a. reachable a \<and> \<not> empty a}" "\<not> empty x"
     shows "\<exists> x' \<in> passed. x \<preceq> x'"
   proof -
     from \<open>reachable x\<close> have "E\<^sup>*\<^sup>* a\<^sub>0 x" by (simp add: reachable_def)
-    from assms(3) obtain b where "a\<^sub>0 \<preceq> b" "b \<in> passed" unfolding start_subsumed_def by auto
+    have "\<not> empty a\<^sub>0" using \<open>E\<^sup>*\<^sup>* a\<^sub>0 x\<close> assms(5) empty_E_star by blast
+    with assms(3) obtain b where "a\<^sub>0 \<preceq> b" "b \<in> passed" unfolding start_subsumed_def by auto
     have "\<exists>x'. \<exists> x''. E\<^sup>*\<^sup>* b x' \<and> x \<preceq> x' \<and> x' \<preceq> x'' \<and> x'' \<in> passed" if
                      "E\<^sup>*\<^sup>* a x"  "a \<preceq> b"   "b \<preceq> b'"   "b' \<in> passed"
                      "reachable a" "reachable b" for a b b'
@@ -381,7 +410,7 @@ context Search_Space begin
 
   lemmas [intro] = step_reachable
 
-  lemma aux7:
+  private lemma aux7:
     assumes
       "a \<in># wait"
       "set_mset wait \<subseteq> Collect reachable"
@@ -390,11 +419,11 @@ context Search_Space begin
     shows "reachable x"
     using assms by (auto dest: in_diffD)
 
-  lemma aux8:
+  private lemma aux8:
     "x \<in> reachable_subsumed S'"  if "x \<in> reachable_subsumed S" "\<forall>s\<in>S. \<exists>x\<in>S'. s \<preceq> x"
     using that unfolding reachable_subsumed_def by (auto intro: trans)
 
-  lemma aux9:
+  private lemma aux9:
     assumes
       "set_mset wait' \<subseteq> set_mset (wait - {#a#}) \<union> Collect (E a)"
       "x \<in># wait'" "\<forall>a'. E a a' \<longrightarrow> \<not> F a'" "F x"
@@ -407,76 +436,82 @@ context Search_Space begin
       by auto
   qed
 
+  private lemma aux10:
+    assumes "\<forall>a\<in>passed' \<union> set_mset wait. \<not> F a" "F x" "x \<in># wait - {#a#}"
+    shows "False"
+    by (meson UnI2 assms in_diffD)
+
+  (* XXX Move and rename *)
+  lemma aux12:
+    "size wait' < size wait" if "wait' \<subseteq># wait - {#a#}" "a \<in># wait"
+    using that
+    by (metis
+        Diff_eq_empty_iff_mset add_diff_cancel_left' add_mset_add_single add_mset_not_empty
+        insert_subset_eq_iff mset_le_add_mset_decr_left1 mset_subset_size subset_mset_def)
+
+  lemma aux13:
+    assumes
+    "passed \<subseteq> {a. reachable a \<and> \<not> empty a}"
+    "passed' \<subseteq> insert a (passed \<union> {a'. E a a' \<and> \<not> empty a'})"
+    "\<not> empty a"
+    "reachable a"
+    "\<forall>s\<in>passed. \<exists>x\<in>passed'. s \<preceq> x"
+    "a'' \<in> passed'"
+    "\<forall>x\<in>passed. \<not> a'' \<preceq> x"
+    shows
+    "passed' \<subseteq> {a. reachable a \<and> \<not> empty a} \<and> reachable_subsumed passed \<subset> reachable_subsumed passed'
+     \<or> passed' = passed \<and> size wait'' < size wait"
+  proof -
+    have "passed' \<subseteq> {a. reachable a \<and> \<not> empty a}"
+      using \<open>passed \<subseteq> _\<close> \<open>passed' \<subseteq> _\<close> \<open>\<not> empty a\<close> \<open>reachable a\<close> by auto
+    moreover have "reachable_subsumed passed \<subset> reachable_subsumed passed'"
+      unfolding reachable_subsumed_def apply auto
+      subgoal
+        using \<open>\<forall>s\<in>passed. \<exists>x\<in>passed'. s \<preceq> x\<close> by (auto intro: trans)
+      using assms(5-) \<open>passed' \<subseteq> {a. reachable a \<and> \<not> empty a}\<close> by auto
+    ultimately show ?thesis
+      using \<open>passed \<subseteq> _\<close> unfolding pw_var_def by auto
+  qed
+
+  method solve_vc =
+    rule aux3 aux5 aux7 aux10 aux11 pw_inv_frontier_empty_elem; assumption; fail |
+    rule aux3; auto; fail | auto intro: aux9; fail | auto dest: in_diffD; fail
+
   theorem pw_algo_correct:
     "pw_algo \<le> SPEC (\<lambda> brk. brk \<longleftrightarrow> F_reachable)"
   proof -
     note [simp] = size_Diff_submset pred_not_lt_is_zero
     note [dest] = set_mset_mp
     show ?thesis
-    unfolding pw_algo_def init_pw_spec_def add_pw_spec_def F_reachable_def
+      unfolding pw_algo_def init_pw_spec_def add_pw_spec_def F_reachable_def
       apply (refine_vcg wf_worklist_var)
-      (* F a\<^sub>0*)
-      apply (auto; fail)
-      (* Invar start*)
-      apply (auto simp: pw_inv_def pw_inv_frontier_def start_subsumed_def; fail)
-      (* Precondition for take-from-set *)
-      apply (simp; fail)
-      (* State is subsumed by passed*)
-        (* Assertion *)
-        apply (auto simp: pw_inv_def; fail)
-        (*Invariant*)
-      subgoal for _ passed _ wait brk _ a wait'
-      apply (clarsimp simp: pw_inv_def split: if_split_asm)
-      apply safe
-        apply (auto dest: in_diffD; fail)+
-          subgoal
-            by (rule aux3; auto)
-          subgoal
-            by (auto dest: in_diffD; fail)
-          subgoal
-            by (auto intro: aux9)
-          subgoal
-            by (rule aux5; auto)
-          subgoal
-            by (rule aux7; auto)
-          subgoal
-            by (rule aux3; auto)
-          subgoal
-            by (auto dest: in_diffD; fail)
-          subgoal
-            by (auto intro: aux9)
-          subgoal
-            by (rule aux5; auto)
-          apply (simp add: aux7)
-          subgoal
-            by (auto dest: in_diffD; fail)
-          done
-        (*Variant*)
-        subgoal for  _ _ _ _ passed _ wait brk _ a wait'
-          apply (clarsimp simp: pw_inv_def split: if_split_asm)
-          apply safe
-            apply (auto; fail)
-          subgoal premises prems for passed' wait'' brk' a' a''
-          proof -
-            have "passed' \<subseteq> Collect reachable"
-              using prems by auto
-            moreover have "reachable_subsumed passed \<subset> reachable_subsumed passed'"
-              unfolding reachable_subsumed_def apply auto
+        (* F a\<^sub>0*)
+               apply (auto; fail)
+        (* empty a\<^sub>0 *)
               subgoal
-                using \<open>\<forall>s\<in>passed. \<exists>x\<in>passed'. s \<preceq> x\<close> by (auto intro: trans)
-              using prems(22-) \<open>passed' \<subseteq> Collect reachable\<close> by auto
-            ultimately show ?thesis
-              using \<open>passed \<subseteq> _\<close> unfolding pw_var_def by auto
-          qed
-          subgoal premises prems for passed' wait'' brk'
-            unfolding pw_var_def
-            using \<open>wait'' \<subseteq># _\<close> Diff_eq_empty_iff_mset mset_subset_size prems(12) subset_mset_def
-            by fastforce
-          subgoal for passed' wait'' brk'
-            unfolding pw_var_def by auto
-          done
-      (* I \<and> \<not> b \<longrightarrow> post *)
-      using F_mono by (fastforce simp: pw_inv_def dest!: aux4)
+                using empty_E_star final_non_empty reachable_def by auto
+        (* Invar start*)
+             apply (fastforce simp: pw_inv_def pw_inv_frontier_def start_subsumed_def
+                              split: if_split_asm dest: mset_subset_eqD)
+        (* Precondition for take-from-set *)
+            apply (simp; fail)
+        (* State is subsumed by passed*)
+        (* Assertion *)
+           apply (auto simp: pw_inv_def; fail)
+        (* Invariant for picking an empty wait list element *)
+          subgoal for _ passed wait _ passed' _ _ brk _ a wait'
+            by (clarsimp simp: pw_inv_def split: if_split_asm; safe; solve_vc)
+        (* Termination for picking an empty wait list element *)
+         apply (clarsimp simp: pw_var_def nonempty_has_size; fail)
+        (* Invariant for picking a non-empty wait list element *)
+        subgoal for _ passed wait _ passed' _ _ brk _ a wait'
+          by (clarsimp simp: pw_inv_def split: if_split_asm; safe; solve_vc) (* slow *)
+        (* Termination for picking a non-empty wait list element *)
+        subgoal for  _ _ _ _ passed _ wait brk _ a wait'
+          by (clarsimp simp: pw_inv_def split: if_split_asm; safe)
+             (simp_all add: aux12 aux13 pw_var_def)
+        (* I \<and> \<not> b \<longrightarrow> post *)
+        using F_mono by (fastforce simp: pw_inv_def dest!: aux4 dest: final_non_empty)
   qed
 
   lemmas [refine_vcg] = pw_algo_correct[THEN order_trans]
